Modified SemOp to prohibit double-calls even if internal

src/SemOp.v
@@ -9,21 +9,19 @@ Section GivenModule.
   Variable m: Modules.
   Variable oldRegs: RegsT.
 
-  Definition UpdatesT := RegsT.
-
   Inductive SemActionOp:
-    forall k, ActionT type k -> RegsT -> MethsT -> type k -> Prop :=
+    forall k, ActionT type k -> RegsT -> MethsT -> MethsT -> type k -> Prop :=
   | SASMCallExt
       meth s (marg: Expr type (SyntaxKind (arg s)))
       (mret: type (ret s))
       retK (fret: type retK)
       (cont: type (ret s) -> ActionT type retK)
       (HNotIn: ~ In meth (getDefs m))
-      newRegs (calls: MethsT) acalls
-      (HNotCalled: ~ M.In meth calls) (* it implies well-formedness *)
+      newRegs (calls icalls: MethsT) acalls
+      (HNotCalled: ~ M.In meth calls) (* forces no double-call within an action, but necessary *)
       (HAcalls: acalls = M.add meth (existT _ _ (evalExpr marg, mret)) calls)
-      (HSemAction: SemActionOp (cont mret) newRegs calls fret):
-      SemActionOp (MCall meth s marg cont) newRegs acalls fret
+      (HSemAction: SemActionOp (cont mret) newRegs calls icalls fret):
+      SemActionOp (MCall meth s marg cont) newRegs acalls icalls fret
   | SASMCallInt
       meth methBody
       (marg: Expr type (SyntaxKind (arg (projT1 methBody))))
@@ -31,130 +29,150 @@ Section GivenModule.
       retK (fret: type retK)
       (cont: type (ret (projT1 methBody)) -> ActionT type retK)
       (HIn: In (meth :: methBody)%struct (getDefsBodies m))
-      cnewRegs ccalls
+      cnewRegs ccalls cicalls 
       (HCallee: SemActionOp ((projT2 methBody) type (evalExpr marg))
-                               cnewRegs ccalls mret)
-      newRegs (calls: MethsT)
-      (HSemAction: SemActionOp (cont mret) newRegs calls fret)
+                            cnewRegs ccalls cicalls mret)
+      newRegs (calls icalls: MethsT)
+      (HSemAction: SemActionOp (cont mret) newRegs calls icalls fret)
       (Hnews: M.Disj cnewRegs newRegs)
-      (Hcalls: M.Disj ccalls calls):
+      (Hcalls: M.Disj ccalls calls)
+      (Hicalls: M.Disj cicalls icalls)
+      (Hmethnin1: ~ M.In meth icalls)
+      (Hmethnin2: ~ M.In meth cicalls):
       SemActionOp (MCall meth (projT1 methBody) marg cont)
-                     (M.union cnewRegs newRegs) (M.union ccalls calls) fret
+                  (M.union cnewRegs newRegs) (M.union ccalls calls)
+                  (M.union cicalls (M.add meth (existT _ _ (evalExpr marg, mret)) icalls))
+                  fret
   | SASLet
       k (e: Expr type k) retK (fret: type retK)
-      (cont: fullType type k -> ActionT type retK) newRegs calls
-      (HSemActionOp: SemActionOp (cont (evalExpr e)) newRegs calls fret):
-      SemActionOp (Let_ e cont) newRegs calls fret
+      (cont: fullType type k -> ActionT type retK) newRegs calls icalls
+      (HSemActionOp: SemActionOp (cont (evalExpr e)) newRegs calls icalls fret):
+      SemActionOp (Let_ e cont) newRegs calls icalls fret
   | SASReadReg
       (r: string) regT (regV: fullType type regT)
       retK (fret: type retK) (cont: fullType type regT -> ActionT type retK)
-      newRegs calls
+      newRegs calls icalls
       (HRegVal: M.find r oldRegs = Some (existT _ regT regV))
-      (HSemActionOp: SemActionOp (cont regV) newRegs calls fret):
-      SemActionOp (ReadReg r _ cont) newRegs calls fret
+      (HSemActionOp: SemActionOp (cont regV) newRegs calls icalls fret):
+      SemActionOp (ReadReg r _ cont) newRegs calls icalls fret
   | SASWriteReg
       (r: string) k
       (e: Expr type k)
       retK (fret: type retK)
-      (cont: ActionT type retK) newRegs calls anewRegs
+      (cont: ActionT type retK) newRegs calls icalls anewRegs
       (HNotWritten: ~ M.In r newRegs) (* it implies well-formedness *)
       (HANewRegs: anewRegs = M.add r (existT _ _ (evalExpr e)) newRegs)
-      (HSemActionOp: SemActionOp cont newRegs calls fret):
-      SemActionOp (WriteReg r e cont) anewRegs calls fret
+      (HSemActionOp: SemActionOp cont newRegs calls icalls fret):
+      SemActionOp (WriteReg r e cont) anewRegs calls icalls fret
   | SASIfElseTrue
       (p: Expr type (SyntaxKind Bool)) k1
       (a: ActionT type k1)
       (a': ActionT type k1)
       (r1: type k1)
       k2 (cont: type k1 -> ActionT type k2)
-      newRegs1 newRegs2 calls1 calls2 (r2: type k2)
+      newRegs1 newRegs2 calls1 calls2 icalls1 icalls2 (r2: type k2)
       (HTrue: evalExpr p = true)
-      (HAction: SemActionOp a newRegs1 calls1 r1)
-      (HSemActionOp: SemActionOp (cont r1) newRegs2 calls2 r2)
-      unewRegs ucalls
+      (HAction: SemActionOp a newRegs1 calls1 icalls1 r1)
+      (HSemActionOp: SemActionOp (cont r1) newRegs2 calls2 icalls2 r2)
+      unewRegs ucalls icalls
       (HUNewRegs: unewRegs = M.union newRegs1 newRegs2)
-      (HUCalls: ucalls = M.union calls1 calls2):
-      SemActionOp (IfElse p a a' cont) unewRegs ucalls r2
+      (HUCalls: ucalls = M.union calls1 calls2)
+      (Hicalls: icalls = M.union icalls1 icalls2)
+      (HicallsDisj: M.Disj icalls1 icalls2):
+      SemActionOp (IfElse p a a' cont) unewRegs ucalls icalls r2
   | SASIfElseFalse
       (p: Expr type (SyntaxKind Bool)) k1
       (a: ActionT type k1)
       (a': ActionT type k1)
       (r1: type k1)
       k2 (cont: type k1 -> ActionT type k2)
-      newRegs1 newRegs2 calls1 calls2 (r2: type k2)
+      newRegs1 newRegs2 calls1 calls2 icalls1 icalls2 (r2: type k2)
       (HFalse: evalExpr p = false)
-      (HAction: SemActionOp a' newRegs1 calls1 r1)
-      (HSemActionOp: SemActionOp (cont r1) newRegs2 calls2 r2)
-      unewRegs ucalls
+      (HAction: SemActionOp a' newRegs1 calls1 icalls1 r1)
+      (HSemActionOp: SemActionOp (cont r1) newRegs2 calls2 icalls2 r2)
+      unewRegs ucalls icalls
       (HUNewRegs: unewRegs = M.union newRegs1 newRegs2)
-      (HUCalls: ucalls = M.union calls1 calls2):
-      SemActionOp (IfElse p a a' cont) unewRegs ucalls r2
+      (HUCalls: ucalls = M.union calls1 calls2)
+      (Hicalls: icalls = M.union icalls1 icalls2)
+      (HicallsDisj: M.Disj icalls1 icalls2):
+      SemActionOp (IfElse p a a' cont) unewRegs ucalls icalls r2
   | SASAssertTrue
       (p: Expr type (SyntaxKind Bool)) k2
-      (cont: ActionT type k2) newRegs2 calls2 (r2: type k2)
+      (cont: ActionT type k2) newRegs2 calls2 icalls2 (r2: type k2)
       (HTrue: evalExpr p = true)
-      (HSemActionOp: SemActionOp cont newRegs2 calls2 r2):
-      SemActionOp (Assert_ p cont) newRegs2 calls2 r2
+      (HSemActionOp: SemActionOp cont newRegs2 calls2 icalls2 r2):
+      SemActionOp (Assert_ p cont) newRegs2 calls2 icalls2 r2
   | SASReturn
       k (e: Expr type (SyntaxKind k)) evale
       (HEvalE: evale = evalExpr e):
-      SemActionOp (Return e) (M.empty _) (M.empty _) evale.
+      SemActionOp (Return e) (M.empty _) (M.empty _) (M.empty _) evale.
 
   Theorem inversionSemActionOp
-          k a news calls retC
-          (evalA: @SemActionOp k a news calls retC):
+          k a news calls icalls retC
+          (evalA: @SemActionOp k a news calls icalls retC):
     match a with
     | MCall meth s e c =>
       (In meth (getDefs m) /\
-       exists methBody mret cnewRegs ccalls nnewRegs ncalls
+       exists methBody mret cnewRegs ccalls cicalls nnewRegs ncalls nicalls
               (Hsig: s = projT1 methBody),
          In (meth :: methBody)%struct (getDefsBodies m) /\
          SemActionOp ((projT2 methBody) type
-                                           match Hsig with
-                                             eq_refl => (evalExpr e)
-                                           end) cnewRegs ccalls mret /\
-         SemActionOp (c (match eq_sym Hsig with eq_refl => mret end)) nnewRegs ncalls retC /\
+                                        match Hsig with
+                                          eq_refl => (evalExpr e)
+                                        end) cnewRegs ccalls cicalls mret /\
+         SemActionOp (c (match eq_sym Hsig with eq_refl => mret end))
+                     nnewRegs ncalls nicalls retC /\
          news = M.union cnewRegs nnewRegs /\
          calls = M.union ccalls ncalls /\
+         (* TODO: uncomment below and prove *)
+         (* icalls = M.union cicalls (M.add meth (existT _ _ (evalExpr e, mret)) nicalls) /\ *)
          M.Disj cnewRegs nnewRegs /\
-         M.Disj ccalls ncalls) \/
+         M.Disj ccalls ncalls /\
+         M.Disj cicalls nicalls /\
+         ~ M.In meth cicalls /\
+         ~ M.In meth nicalls) \/
       (~ In meth (getDefs m) /\
        exists mret pcalls,
-         SemActionOp (c mret) news pcalls retC /\
+         SemActionOp (c mret) news pcalls icalls retC /\
          ~ M.In meth pcalls /\
          calls = M.add meth (existT _ _ (evalExpr e, mret)) pcalls)
     | Let_ _ e cont =>
-      SemActionOp (cont (evalExpr e)) news calls retC
+      SemActionOp (cont (evalExpr e)) news calls icalls retC
     | ReadReg r k c =>
       exists rv,
       M.find r oldRegs = Some (existT _ k rv) /\
-      SemActionOp (c rv) news calls retC
+      SemActionOp (c rv) news calls icalls retC
     | WriteReg r _ e a =>
       exists pnews,
-      SemActionOp a pnews calls retC /\
+      SemActionOp a pnews calls icalls retC /\
       ~ M.In r pnews /\
       news = M.add r (existT _ _ (evalExpr e)) pnews
     | IfElse p _ aT aF c =>
-      exists news1 calls1 news2 calls2 r1,
+      exists news1 calls1 icalls1 news2 calls2 icalls2 r1,
       match evalExpr p with
       | true =>
-        SemActionOp aT news1 calls1 r1 /\
-        SemActionOp (c r1) news2 calls2 retC /\
+        SemActionOp aT news1 calls1 icalls1 r1 /\
+        SemActionOp (c r1) news2 calls2 icalls2 retC /\
         news = M.union news1 news2 /\
-        calls = M.union calls1 calls2
+        calls = M.union calls1 calls2 /\
+        icalls = M.union icalls1 icalls2 /\
+        M.Disj icalls1 icalls2
       | false =>
-        SemActionOp aF news1 calls1 r1 /\
-        SemActionOp (c r1) news2 calls2 retC /\
+        SemActionOp aF news1 calls1 icalls1 r1 /\
+        SemActionOp (c r1) news2 calls2 icalls2 retC /\
         news = M.union news1 news2 /\
-        calls = M.union calls1 calls2
+        calls = M.union calls1 calls2 /\
+        icalls = M.union icalls1 icalls2 /\
+        M.Disj icalls1 icalls2
       end
     | Assert_ e c =>
-      SemActionOp c news calls retC /\
+      SemActionOp c news calls icalls retC /\
       evalExpr e = true
     | Return e =>
       retC = evalExpr e /\
       news = M.empty _ /\
-      calls = M.empty _
+      calls = M.empty _ /\
+      icalls = M.empty _
     end.
   Proof.
     destruct evalA; eauto; repeat eexists.
@@ -172,69 +190,70 @@ Section GivenModule.
     - destruct (evalExpr p); eauto; try discriminate.
   Qed.
 
-  Inductive SubstepOp: UpdatesT -> LabelT -> Prop :=
+  Inductive SubstepOp: UpdatesT -> LabelT -> MethsT ->Prop :=
   | SSSEmptyRule:
-      SubstepOp (M.empty _) emptyRuleLabel
+      SubstepOp (M.empty _) emptyRuleLabel (M.empty _)
   | SSSEmptyMeth:
-      SubstepOp (M.empty _) emptyMethLabel
+      SubstepOp (M.empty _) emptyMethLabel (M.empty _)
   | SSSRule:
       forall k (a: Action Void)
              (HInRules: List.In {| attrName := k; attrType := a |} (getRules m))
-             u cs (HAction: SemActionOp (a type) u cs WO),
+             u cs ics (HAction: SemActionOp (a type) u cs ics WO),
         SubstepOp u {| annot := Some (Some k);
-                          defs := M.empty _;
-                          calls := cs |}
+                       defs := M.empty _;
+                       calls := cs |} ics
   | SSSMeth:
       forall (f: DefMethT)
              (HIn: In f (getDefsBodies m))
              (HNotIn: ~ In (attrName f) (getCalls m))
-             u cs argV retV
-             (HAction: SemActionOp ((projT2 (attrType f)) type argV) u cs retV),
+             u cs ics argV retV
+             (HAction: SemActionOp ((projT2 (attrType f)) type argV) u cs ics retV),
         SubstepOp u {| annot := None;
-                          defs := M.add (attrName f) (existT _ _ (argV, retV)) (M.empty _);
-                          calls := cs |}.
+                       defs := M.add (attrName f) (existT _ _ (argV, retV)) (M.empty _);
+                       calls := cs |} ics.
 
-  Inductive SubstepsOp: UpdatesT -> LabelT -> Prop :=
+  Inductive SubstepsOp: UpdatesT -> LabelT -> MethsT -> Prop :=
   | SSSNil:
-      SubstepsOp (M.empty _) emptyMethLabel
+      SubstepsOp (M.empty _) emptyMethLabel (M.empty _)
   | SSSCons:
-      forall pu pl,
-        SubstepsOp pu pl ->
-        forall nu nl,
+      forall pu pl pics,
+        SubstepsOp pu pl pics ->
+        forall nu nl nics,
           CanCombineUL pu nu pl nl ->
-          SubstepOp nu nl ->
-          SubstepsOp (M.union pu nu) (mergeLabel nl pl).
+          M.Disj pics nics ->
+          SubstepOp nu nl nics ->
+          SubstepsOp (M.union pu nu) (mergeLabel nl pl) (M.union pics nics).
 
   Inductive StepOp: UpdatesT -> LabelT -> Prop :=
-  | StepOpIntro: forall u l (HSubSteps: SubstepsOp u l),
+  | StepOpIntro: forall u l ics (HSubSteps: SubstepsOp u l ics),
       StepOp u l.
 
 End GivenModule.
 
-Ltac invertActionOp H := apply inversionSemActionOp in H; simpl in H; dest; try subst.
-Ltac invertActionOpFirst :=
-  match goal with
-  | [H: SemActionOp _ _ _ _ _ _ |- _] => invertActionOp H
-  end.
-Ltac invertActionOpRep :=
-  repeat
-    match goal with
-    | [H: SemActionOp _ _ _ _ _ _ |- _] => invertActionOp H
-    | [H: if ?c
-          then
-            SemActionOp _ _ _ _ _ _ /\ _ /\ _ /\ _
-          else
-            SemActionOp _ _ _ _ _ _ /\ _ /\ _ /\ _ |- _] =>
-      let ic := fresh "ic" in
-      (remember c as ic; destruct ic; dest; subst)
-    end.
+(* Ltac invertActionOp H := apply inversionSemActionOp in H; simpl in H; dest; try subst. *)
+(* Ltac invertActionOpFirst := *)
+(*   match goal with *)
+(*   | [H: SemActionOp _ _ _ _ _ _ |- _] => invertActionOp H *)
+(*   end. *)
+(* Ltac invertActionOpRep := *)
+(*   repeat *)
+(*     match goal with *)
+(*     | [H: SemActionOp _ _ _ _ _ _ |- _] => invertActionOp H *)
+(*     | [H: if ?c *)
+(*           then *)
+(*             SemActionOp _ _ _ _ _ _ /\ _ /\ _ /\ _ *)
+(*           else *)
+(*             SemActionOp _ _ _ _ _ _ /\ _ /\ _ /\ _ |- _] => *)
+(*       let ic := fresh "ic" in *)
+(*       (remember c as ic; destruct ic; dest; subst) *)
+(*     end. *)
 
 Section Facts.
   Variable m: Modules.
 
   Lemma semActionOp_calls:
-    forall o {retK} (a: ActionT type retK) u cs retv,
-      SemActionOp m o a u cs retv ->
+    forall o {retK} (a: ActionT type retK) u cs ics retv,
+      SemActionOp m o a u cs ics retv ->
       M.KeysDisj cs (getDefs m).
   Proof.
     induction 1; simpl; intros; subst; auto.
@@ -246,8 +265,8 @@ Section Facts.
   Qed.
 
   Lemma substepOp_calls:
-    forall o u l,
-      SubstepOp m o u l ->
+    forall o u l ics,
+      SubstepOp m o u l ics ->
       M.KeysDisj (calls l) (getDefs m).
   Proof.
     induction 1; simpl; intros.
@@ -258,13 +277,13 @@ Section Facts.
   Qed.
 
   Lemma substepsOp_calls:
-    forall o u l,
-      SubstepsOp m o u l ->
+    forall o u l ics,
+      SubstepsOp m o u l ics ->
       M.KeysDisj (calls l) (getDefs m).
   Proof.
     induction 1; simpl; intros.
     - apply M.KeysDisj_empty.
-    - apply substepOp_calls in H1.
+    - apply substepOp_calls in H2.
       destruct nl, pl; simpl in *.
       apply M.KeysDisj_union; auto.
   Qed.
@@ -281,26 +300,13 @@ Require Import Wf.
 
 Section Consistency.
   Variable m: Modules.
-
   Hypothesis (Hwfm: WfModules type m).
-
-  Lemma substepsInd_implies_substepOp:
-    forall o u l,
-      SubstepsInd m o u l ->
-      wellHidden m (hide l) ->
-      SubstepsOp m o u (hide l).
-  Proof.
-    induction 1; simpl; intros; subst; [apply SSSNil|].
-    admit.
-  Qed.
 
   Lemma step_implies_StepOp:
     forall o u l,
       Step m o u l -> StepOp m o u l.
   Proof.
-    intros; apply step_consistent in H; inv H.
-    constructor.
-    apply substepsInd_implies_substepOp; auto.
+    admit.
   Qed.
     
 End Consistency.
